\documentclass[12pt]{article}

\usepackage[margin=1in]{geometry}

\usepackage{logictextbook}

\title{Zeroth-order logic tableau rule sheet}
\author{Peter Susanszky: Learning Logic Backwards}
\date{}

\begin{document}
\maketitle
\centering

\begin{tabular}{cc}
\parbox{0.5\textwidth}{\centering{\fbox{
	\begin{prooftree}{}
		[{X\wedge Y}
		[{X}, just=$\wedge$:!u]
		]
\end{prooftree}}

\fbox{
	\begin{prooftree}{}
		[{X\wedge Y}
		[{Y}, just=$\wedge$:!u]
		]
\end{prooftree}}
}}
&
\parbox{0.5\textwidth}{\centering\fbox{
	\begin{prooftree}{}
		[{\neg (X\vee Y)}
		[{\neg X}, just=$\neg\vee$:!u]
		]
\end{prooftree}}

\fbox{
	\begin{prooftree}{}
		[{\neg(X\vee Y)}
		[{\neg Y}, just=$\neg\vee$:!u]
		]
\end{prooftree}}
}
\\
$\wedge$: Conjunction rule& $\neg \vee$: Negated disjunction rule\\
\end{tabular}

\begin{center}
\fbox{
		\begin{prooftree}{}
			[{\neg (X\rightarrow Y)}
			[{X}, just=$\neg\rightarrow$:!u]
			]
		\end{prooftree}}

\fbox{
		\begin{prooftree}{}
			[{\neg(X\rightarrow Y)}
			[{\neg Y}, just=$\neg\rightarrow$:!u]
			]
		\end{prooftree}}


\medskip
$\neg\rightarrow$: Negated conditional rule
\end{center}

\begin{tabular}{cc}
\parbox{0.5\textwidth}{\centering\fbox{
	\begin{prooftree}{}
		[{X\vee Y}
		[{X}, just=$\vee$:!u]
		[{Y}]
		]
	\end{prooftree}}}
&
\parbox{0.5\textwidth}{\centering\fbox{
	\begin{prooftree}{}
		[{\neg (X\wedge Y)}
		[{\neg X}, just=$\neg\wedge$:!u]
		[{\neg Y}]
		]
	\end{prooftree}}}

\\
$\vee$:	Disjunction rule & $\neg\wedge$: Negated conjunction rule\\
\parbox{0.5\textwidth}{\centering\fbox{
	\begin{prooftree}{}
		[{X \rightarrow Y}
		[{\neg X}, just=$\rightarrow$:!u]
		[{Y}]
		]
	\end{prooftree}}}
&
\parbox{0.5\textwidth}{\centering\fbox{
	\begin{prooftree}{}
		[{\neg\neg X}
		[{X}, just=$\neg\neg$:!u]
		]
	\end{prooftree}}}
\\
$\rightarrow$: Conditional rule& $\neg\neg$: Double negation rule
\end{tabular}

\end{document}